tweaked smallfilter some more

deps/poulet4/lib/P4automata/Benchmarks/SmallFilterProof.v
@@ -6,18 +6,44 @@ Notation H := (IncrementalBits.header + BigBits.header).
 Notation A := IncrementalSeparate.aut.
 Notation conf := (P4automaton.configuration (P4A.interp A)).
 
-Definition r_states :=
-  Eval vm_compute in (Reachability.reachable_states
-                        IncrementalSeparate.aut
-                        200
-                        IncrementalBits.Start
-                        BigBits.Parse).
+Definition r_states' := (Reachability.reachable_states
+                          IncrementalSeparate.aut
+                          200
+                          IncrementalBits.Start
+                          BigBits.Parse).
+
+Definition r_states := Eval vm_compute in r_states'.
 
 Definition top : Relations.rel conf :=
   fun q1 q2 => List.In (conf_to_state_template q1, conf_to_state_template q2) r_states.
 
 Definition top' : Relations.rel (state_template A) :=
   fun q1 q2 => List.In (q1, q2) r_states.
+
+Definition top'' : Relations.rel conf :=
+  fun q1 q2 => List.In (conf_to_state_template q1, conf_to_state_template q2) r_states'.
+
+Definition top''' : Relations.rel (state_template A) :=
+  fun q1 q2 => List.In (q1, q2) r_states'.
+
+Lemma r_states_conv: 
+  r_states = r_states'.
+Proof.
+  vm_compute.
+  exact eq_refl.
+Qed.
+
+Lemma top_conv: 
+  forall q1 q2, top q1 q2 <-> top'' q1 q2.
+Proof.
+  intros; unfold top, top''; erewrite r_states_conv; eapply iff_refl.
+Qed.
+
+Lemma top'_conv: 
+  forall q1 q2, top' q1 q2 <-> top''' q1 q2.
+Proof.
+  intros; unfold top', top'''; erewrite r_states_conv; eapply iff_refl.
+Qed.
 
 Declare ML Module "mirrorsolve".
 
@@ -60,5 +86,42 @@ Proof.
   subst rel0.
 
   time "build phase" repeat (time "single step" run_bisim top top' r_states).
-  time "close phase" close_bisim' top'.
+
+  eapply PreBisimulationClose;
+  match goal with
+  | H: interp_conf_rel' ?C ?q1 ?q2|- interp_crel _ ?top ?P ?q1 ?q2 =>
+    let H0 := fresh "H0" in
+    assert (H0: interp_entailment' top {| e_prem := P; e_concl := C |}) by (
+      eapply simplify_entailment_correct' with (i := top');
+      eapply compile_simplified_entailment_correct';
+
+      simpl; intros;
+      eapply FirstOrderConfRelSimplified.simplify_eq_zero_fm_corr;
+      eapply CompileFirstOrderConfRelSimplified.compile_simplified_fm_bv_correct;
+
+      crunch_foterm;
+      match goal with
+      | |- ?X => time "smt check pos" check_interp_pos X; admit
+      end
+    );
+    eapply H0;
+    destruct q1, q2;
+    vm_compute in H;
+    repeat match goal with 
+    | H: _ /\ _ |- _ => destruct H
+    end;
+    [
+      (* apply in_checker_conv with (A_eq := fun x y => state_temp_prod_eqdec x y);
+      unfold conf_to_state_template, P4automaton.conf_buf_len, P4automaton.conf_state;
+    
+      repeat match goal with 
+      | H: _ = _ |- _ => erewrite <- H
+      end;
+      exact eq_refl *)
+                    |
+      split; [ vm_compute; (repeat split || assumption) | (intros; exact I)]
+    ] 
+  end.
+    eapply top_conv.
+    unfold top''.
 Time Admitted.
